hol/pred_specScript.sml
@@ -77,14 +77,15 @@ Definition mk_substitute_pred_def:
   (mk_substitute_pred (True) x b = True) ∧
   (mk_substitute_pred (False) x b = False) ∧
   (mk_substitute_pred (Var x') x b = 
-  if (x=x') then (if b then True else False) else (Var x') 
-  ) ∧
+   if (x=x') then (if b then True else False) else (Var x')) ∧
   (mk_substitute_pred (And c c' ) x b =
-      (And (mk_substitute_pred c x b) (mk_substitute_pred c' x b ))) ∧
+   (And (mk_substitute_pred c x b) (mk_substitute_pred c' x b ))) ∧
   (mk_substitute_pred (Or c c') x b =
-      (Or (mk_substitute_pred c x b) (mk_substitute_pred c' x b ))) ∧
+   (Or (mk_substitute_pred c x b) (mk_substitute_pred c' x b ))) ∧
   (mk_substitute_pred (Not c) x b=
-      (Not (mk_substitute_pred c x b)))
+   (Not (mk_substitute_pred c x b))) ∧
+  (mk_substitute_pred (Implies c c') x b =
+   (Implies (mk_substitute_pred c x b) (mk_substitute_pred c' x b )))
 End
 
 
@@ -134,14 +135,27 @@ End
    
 
 
-Definition pred_final_def:
- pred_final p = 
- case p of
- | True => SOME T
- | False => SOME F
- | _ => NONE
+Definition final_pred_def:
+  final_pred p = 
+  case p of
+  | True => SOME T
+  | False => SOME F
+  | _ => NONE
 End
-                                                                
+
+
+
+Definition fv_pred_def:
+  fv_pred (Var x) = [x] ∧
+  fv_pred True = [] ∧
+  fv_pred False = [] ∧
+  fv_pred (And p q) = nub (fv_pred p ++ fv_pred q) ∧
+  fv_pred (Or p q) = nub (fv_pred p ++ fv_pred q) ∧
+  fv_pred (Not p) = fv_pred p ∧
+  fv_pred (Implies p q) = nub (fv_pred p ++ fv_pred q)
+End
+
+        
                                                          
 Definition pred_structure_def:
   pred_structure =
@@ -149,42 +163,30 @@ Definition pred_structure_def:
     sem := sem_pred;
     sub := mk_substitute_pred;
     simp := simp_pred;
-    final := pred_final;
+    final := final_pred;
+    fv := fv_pred;
   |>
 End            
-
-                                           
-       
-
-Definition FV_def:
-  FV (Var x) = [x] ∧
-  FV True = [] ∧
-  FV False = [] ∧
-  FV (And p q) = nub (FV p ++ FV q) ∧
-  FV (Or p q) = nub (FV p ++ FV q) ∧
-  FV (Not p) = FV p ∧
-  FV (Implies p q) = nub (FV p ++ FV q)
-End
-
-
 
 
 Theorem simp_pred_imp_mem:          
   ∀ p x .
     simp_pred p = Var x ⇒
-    MEM x (FV p)
+    MEM x (fv_pred p)
 Proof
   Induct >>
-  rw[simp_pred_def, FV_def] >> gvs[AllCaseEqs()]
+  rw[simp_pred_def, fv_pred_def] >> gvs[AllCaseEqs()]
 QED
 
 
+
+        
 Theorem mem_imp_sem_pred:        
-  ∀p mv. (∀x. MEM x (FV p) ⇒ (∃b. ALOOKUP mv x = SOME b)) ⇒
+  ∀p mv. (∀x. MEM x (fv_pred p) ⇒ (∃b. ALOOKUP mv x = SOME b)) ⇒
          sem_pred p mv ≠ NONE ∧ ∃ b' . sem_pred p mv = SOME b'
 Proof
   Induct >>
-  rw[simp_pred_def, FV_def] >> gvs[AllCaseEqs()] >>
+  rw[simp_pred_def, fv_pred_def] >> gvs[AllCaseEqs()] >>
   gvs[sem_pred_def, simp_pred_def] >>
   rpt (BasicProvers.FULL_CASE_TAC >> gvs[]) 
 QED
@@ -193,19 +195,19 @@ QED
 
 
 Theorem simplification_correct:
-  ∀p mv. (∀x. MEM x (FV p) ⇒ (∃b. ALOOKUP mv x = SOME b)) ⇒
+  ∀p mv. (∀x. MEM x (fv_pred p) ⇒ (∃b. ALOOKUP mv x = SOME b)) ⇒
          sem_pred p mv = sem_pred (simp_pred p) mv
 Proof
   Induct_on `p` >-
    (rw[simp_pred_def, sem_pred_def]) >-
    (rw[simp_pred_def, sem_pred_def]) >-
    (rw[simp_pred_def, sem_pred_def]) >>
-
+  
   rpt strip_tac >>
   imp_res_tac mem_imp_sem_pred >>
-
+  
   LAST_X_ASSUM (STRIP_ASSUME_TAC o (Q.SPECL [‘mv’])) >>
-  gvs[FV_def] >>
+  gvs[fv_pred_def] >>
   gvs[sem_pred_def] >>   
 
   rw[sem_pred_def, simp_pred_def] >>   
@@ -216,7 +218,149 @@ Proof
   imp_res_tac simp_pred_imp_mem >>
   gvs[]
 QED
-           
+
+
+
+
+
+
+
+
+Theorem fv_in_sub_indeed_in_p:   
+  ∀ p h b s.
+    MEM s (fv_pred (mk_substitute_pred p h b)) ⇒
+    MEM s (fv_pred p)
+Proof
+  Induct_on ‘p’ >>
+  (* T, F and Var cases *)
+  gvs[fv_pred_def, mk_substitute_pred_def] >>
+  rpt strip_tac >>
+  rpt (BasicProvers.FULL_CASE_TAC >> gvs[]) >>
+  gvs[fv_pred_def] >>
+  
+  (* rest of cases *)
+  rpt strip_tac >>
+  gvs[mk_substitute_pred_def] >>
+  Cases_on ‘p’ >>
+  gvs[mk_substitute_pred_def] >>
+  rpt (BasicProvers.FULL_CASE_TAC >> gvs[]) >>
+  gvs[fv_pred_def] >>
+  gvs[mk_substitute_pred_def] >>
+  res_tac >>
+  gvs[]
+QED
+        
+
+        
+
+
+Theorem pred_fv_mem_decomposition:        
+  ∀ p p' mv.
+    ((∀x. MEM x (fv_pred (And p p')) ⇒ ∃b. ALOOKUP mv x = SOME b) ∨
+     (∀x. MEM x (fv_pred (Or p p')) ⇒ ∃b. ALOOKUP mv x = SOME b) ∨
+     (∀x. MEM x (fv_pred (Implies p p')) ⇒ ∃b. ALOOKUP mv x = SOME b))⇒
+    ((∀x. MEM x (fv_pred p) ⇒ ∃b'. ALOOKUP mv x = SOME b') ∧
+     (∀x. MEM x (fv_pred p') ⇒ ∃b''. ALOOKUP mv x = SOME b'')) 
+Proof
+  rpt strip_tac >>
+  gvs[fv_pred_def]
+QED
+
+
+
+
+Theorem pred_not_fv_mem_decomposition:        
+  ∀ p p' mv.
+    (∀x. MEM x (fv_pred (Not p)) ⇒ ∃b. ALOOKUP mv x = SOME b )⇒
+    (∀x. MEM x (fv_pred p) ⇒ ∃b'. ALOOKUP mv x = SOME b') 
+Proof
+  rpt strip_tac >>
+  gvs[fv_pred_def]
+QED
+
+        
+
+
+Theorem sem_pred_subst_congruence:
+  ∀ mv p p' x x' b h.
+    ALOOKUP mv h = SOME b ∧
+    sem_pred p mv = SOME x ∧
+    sem_pred p' mv = SOME x' ∧        
+    sem_pred (simp_pred (mk_substitute_pred p' h b)) mv = sem_pred p' mv ∧
+    sem_pred (simp_pred (mk_substitute_pred p h b)) mv = sem_pred p mv ⇒
+    (sem_pred (simp_pred (mk_substitute_pred (And p p') h b)) mv = SOME (x ∧ x') ∧
+     sem_pred (simp_pred (mk_substitute_pred (Or p p') h b)) mv = SOME (x ∨ x') ∧
+     sem_pred (simp_pred (mk_substitute_pred (Implies p p') h b)) mv = SOME (x ⇒ x') ∧
+     sem_pred (simp_pred (mk_substitute_pred (Not p) h b)) mv = SOME (~x)
+    )
+Proof
+  rpt strip_tac >>
+  gvs[mk_substitute_pred_def] >>
+  gvs[simp_pred_def] >>
+  rpt (BasicProvers.FULL_CASE_TAC >> gvs[]) >>
+  gvs[sem_pred_def]
+QED
+
+
+
+Theorem sem_pred_not_subst_congruence:
+  ∀ mv p p' x x' b h.
+    ALOOKUP mv h = SOME b ∧
+    sem_pred p mv = SOME x ∧  
+    sem_pred (simp_pred (mk_substitute_pred p h b)) mv = sem_pred p mv ⇒
+    (sem_pred (simp_pred (mk_substitute_pred (Not p) h b)) mv = SOME (~x))
+Proof
+  rpt strip_tac >>
+  gvs[mk_substitute_pred_def] >>
+  gvs[simp_pred_def] >>
+  rpt (BasicProvers.FULL_CASE_TAC >> gvs[]) >>
+  gvs[sem_pred_def]
+QED
+
+
+        
+
+(* proof of property 1 for predicates *)
+Theorem prop1_pred:
+  prop1 pred_structure
+Proof
+  gvs[prop1_def] >>
+  gvs[fv_in_p_def, pred_structure_def] >>
+  Induct_on ‘p’ >>
+  rpt strip_tac >>~-([‘sem_pred (Var s) mv’],
+                     (gvs[mk_substitute_pred_def] >>
+                      Cases_on ‘h=s’ >> 
+                      gvs[simp_pred_def, sem_pred_def] >>
+                      Cases_on ‘b’ >> gvs[simp_pred_def, sem_pred_def])
+                    ) >>~- ([‘sem_pred True mv’],
+                            gvs[mk_substitute_pred_def] >>
+                            gvs[simp_pred_def]
+                           ) >>~- ([‘sem_pred False mv’],
+                                   gvs[mk_substitute_pred_def] >>
+                                   gvs[simp_pred_def]
+                                  ) >>
+  
+  
+  simp[sem_pred_def] >>
+  rpt (BasicProvers.FULL_CASE_TAC >> gvs[]) >>
+  imp_res_tac mem_imp_sem_pred >>
+  rgs[sem_pred_def] >>
+  gvs[] >>
+  
+  imp_res_tac pred_fv_mem_decomposition >>
+  imp_res_tac pred_not_fv_mem_decomposition >>
+  
+  res_tac >>
+  gvs[sem_pred_subst_congruence, sem_pred_not_subst_congruence]
+QED
+
+
+
+          
+
+
+     
+        
 
 val _ = export_theory ();
 
